WP1-Programming-Languages-Semantics/WP11-C-semantics/src/orca/theories/utp_fault_rea_designs.thy
@@ -1,0 +1,257 @@
+theory utp_fault_rea_designs
+imports  utp_reactive
+begin
+subsection {*Sequential C-program alphabet*}
+
+text {*In order to record the interaction of a sequential C program with its execution environment, 
+       we extend the alphabet of UTP by two additional global state variables:
+      \begin{itemize}   
+       \<^item> fault: a variable of type @{typ "'f option"} used to record a fault of a given guard is 
+         not satisfied.
+       \<^item> abrupt: a boolean variable used to
+     \end{itemize}
+
+*}
+
+alphabet 'f cp_vars = "'t rp_vars" +
+  abrupt:: bool
+  fault :: "'f option"
+  (*wait :: bool*)
+
+declare cp_vars.splits [alpha_splits]
+
+subsubsection {*Alphabet proofs*}
+text {*
+  The two locale interpretations below are a technicality to improve automatic
+  proof support via the predicate and relational tactics. This is to enable the
+  (re-)interpretation of state spaces to remove any occurrences of lens types
+  after the proof tactics @{method pred_simp} and @{method rel_simp}, or any
+  of their derivatives have been applied. Eventually, it would be desirable to
+  automate both interpretations as part of a custom outer command for defining
+  alphabets.
+*}
+
+interpretation cp_vars:
+  lens_interp "\<lambda> (ok, wait, tr, r). 
+  (ok, wait, tr, abrupt\<^sub>v r, fault\<^sub>v r, more r)"
+apply (unfold_locales)
+apply (rule injI)
+apply (clarsimp)
+done
+
+interpretation cp_vars_rel: lens_interp "\<lambda>(ok, ok', wait, tr, wait', tr', r, r').
+  (ok, ok', wait, wait', tr, tr', abrupt\<^sub>v r, abrupt\<^sub>v r', fault\<^sub>v r, fault\<^sub>v r', more r, more r')"
+apply (unfold_locales)
+apply (rule injI)
+apply (clarsimp)
+done
+
+subsubsection {*Type lifting*}
+
+type_synonym ('t, 'f, '\<alpha>) cp = "('t, ('f, '\<alpha>) cp_vars_scheme) rp"
+type_synonym ('t,'f,'\<alpha>,'\<beta>) rel_cp  = "(('t,'f,'\<alpha>) cp, ('t,'f,'\<beta>) cp) rel"
+type_synonym ('t,'f,'\<alpha>) hrel_cp  = "(('t,'f,'\<alpha>) cp) hrel"
+
+subsubsection {*Syntactic type setup*}
+
+translations
+  (type) "('t, 'f, '\<alpha>) cp" <= (type) "('t, ('f, '\<alpha>) cp_vars_scheme) rp_vars_scheme des"
+  (type) "('t, 'f, '\<alpha>) cp" <= (type) "('t, ('f, '\<alpha>) cp_vars_scheme) rp_vars_ext des"
+  (type) "('t, 'f,'\<alpha>,'\<beta>) rel_cp" <= (type) "(('t,'f,'\<alpha>) cp, (_,_,'\<beta>) cp) rel"
+
+notation cp_vars_child_lens\<^sub>a ("\<Sigma>\<^sub>c")
+notation cp_vars_child_lens ("\<Sigma>\<^sub>C")
+
+syntax
+  "_svid_st_alpha"  :: "svid" ("\<Sigma>\<^sub>C")
+  "_svid_st_a"  :: "svid" ("\<Sigma>\<^sub>c")
+translations
+  "_svid_st_alpha" => "CONST cp_vars_child_lens"
+   "_svid_st_a" => "CONST cp_vars_child_lens\<^sub>a"
+
+lemma cvars_ord [usubst]:
+  "$fault \<prec>\<^sub>v $fault\<acute>" "$abrupt \<prec>\<^sub>v $abrupt\<acute>"  "$ok \<prec>\<^sub>v $ok\<acute>"
+  "$ok \<prec>\<^sub>v $wait\<acute>" "$ok \<prec>\<^sub>v $wait" "$ok\<acute> \<prec>\<^sub>v $wait\<acute>"  "$ok\<acute> \<prec>\<^sub>v $wait"
+  "$ok \<prec>\<^sub>v $fault\<acute>" "$ok \<prec>\<^sub>v $fault" "$ok\<acute> \<prec>\<^sub>v $fault\<acute>"  "$ok\<acute> \<prec>\<^sub>v $fault"
+  "$ok \<prec>\<^sub>v $abrupt\<acute>" "$ok \<prec>\<^sub>v $abrupt" "$ok\<acute> \<prec>\<^sub>v $abrupt\<acute>"  "$ok\<acute> \<prec>\<^sub>v $abrupt" 
+  "$fault \<prec>\<^sub>v $abrupt\<acute>" "$fault \<prec>\<^sub>v $abrupt" "$fault\<acute> \<prec>\<^sub>v $abrupt\<acute>"  "$fault\<acute> \<prec>\<^sub>v $abrupt"
+  "$fault \<prec>\<^sub>v $wait\<acute>" "$fault \<prec>\<^sub>v $wait" "$fault\<acute> \<prec>\<^sub>v $wait\<acute>"  "$fault\<acute> \<prec>\<^sub>v $wait"
+  "$abrupt \<prec>\<^sub>v $wait\<acute>" "$abrupt \<prec>\<^sub>v $wait" "$abrupt\<acute> \<prec>\<^sub>v $wait\<acute>"  "$abrupt\<acute> \<prec>\<^sub>v $wait"
+  by (simp_all add: var_name_ord_def)
+
+abbreviation abrupt_f::"('t::ordered_cancel_monoid_diff,'f, '\<alpha>, '\<beta>) rel_cp \<Rightarrow> 
+                        ('t,'f, '\<alpha>, '\<beta>) rel_cp"
+where "abrupt_f R \<equiv> R\<lbrakk>false/$abrupt\<rbrakk>"
+
+abbreviation abrupt_t::"('t::ordered_cancel_monoid_diff,'f, '\<alpha>, '\<beta>) rel_cp \<Rightarrow> 
+                        ('t,'f, '\<alpha>, '\<beta>) rel_cp"
+where "abrupt_t R \<equiv> R\<lbrakk>true/$abrupt\<rbrakk>"
+
+syntax
+  "_abrupt_f"  :: "logic \<Rightarrow> logic" ("_\<^sub>a\<^sub>f" [1000] 1000)
+  "_abrupt_t"  :: "logic \<Rightarrow> logic" ("_\<^sub>a\<^sub>t" [1000] 1000)
+
+translations
+  "P \<^sub>a\<^sub>f" \<rightleftharpoons> "CONST usubst (CONST subst_upd CONST id (CONST ivar CONST abrupt) false) P"
+  "P \<^sub>a\<^sub>t" \<rightleftharpoons> "CONST usubst (CONST subst_upd CONST id (CONST ivar CONST abrupt) true) P"
+
+subsection {*UTP-Relations lift and drop*}
+
+abbreviation lift_desr ("\<lceil>_\<rceil>\<^sub>C")
+where "\<lceil>P\<rceil>\<^sub>C \<equiv> P \<oplus>\<^sub>p (\<Sigma>\<^sub>C \<times>\<^sub>L \<Sigma>\<^sub>C)"
+
+abbreviation lift_pre_desr ("\<lceil>_\<rceil>\<^sub>C\<^sub><")
+where "\<lceil>p\<rceil>\<^sub>C\<^sub>< \<equiv> \<lceil>\<lceil>p\<rceil>\<^sub><\<rceil>\<^sub>C"
+
+abbreviation lift_post_desr ("\<lceil>_\<rceil>\<^sub>C\<^sub>>")
+where "\<lceil>p\<rceil>\<^sub>C\<^sub>> \<equiv> \<lceil>\<lceil>p\<rceil>\<^sub>>\<rceil>\<^sub>C"
+
+abbreviation drop_desr ("\<lfloor>_\<rfloor>\<^sub>C")
+where "\<lfloor>P\<rfloor>\<^sub>C \<equiv> P \<restriction>\<^sub>p (\<Sigma>\<^sub>C \<times>\<^sub>L \<Sigma>\<^sub>C)"
+
+
+subsection {* Reactive lemmas *}
+
+lemma unrest_ok_lift_rea [unrest]:
+  "$ok \<sharp> \<lceil>P\<rceil>\<^sub>C" "$ok\<acute> \<sharp> \<lceil>P\<rceil>\<^sub>C"
+  by (pred_auto)+
+
+lemma unrest_wait_lift_rea [unrest]:
+  "$abrupt \<sharp> \<lceil>P\<rceil>\<^sub>C" "$abrupt\<acute> \<sharp> \<lceil>P\<rceil>\<^sub>C"
+  by (pred_auto)+
+
+lemma unrest_tr_lift_rea [unrest]:
+  "$fault \<sharp> \<lceil>P\<rceil>\<^sub>C" "$fault\<acute> \<sharp> \<lceil>P\<rceil>\<^sub>C"
+  by (pred_auto)+
+
+lemma seqr_wait_true [usubst]: "(P ;; Q) \<^sub>a\<^sub>t = (P \<^sub>a\<^sub>t ;; Q)"
+  by (rel_auto)
+
+lemma seqr_wait_false [usubst]: "(P ;; Q) \<^sub>a\<^sub>f = (P \<^sub>a\<^sub>f ;; Q)"
+  by (rel_auto)
+
+subsection{*Healthiness conditions*}
+text {*In UTP healthiness conditions is away to express invariant on the alphabet.
+       The following healthiness condition express that programs in, wait, fault or 
+       abrupt state do not progress.*}
+definition C3_def [upred_defs]: "C3(P) = 
+           (P \<triangleleft>  \<not>$wait \<and> \<not>$abrupt \<and> $fault =\<^sub>u \<guillemotleft>None\<guillemotright> \<triangleright> II )"
+
+subsection {*exec semantics*}
+text {*We introduce an execution semantics for the designs containing a specific values for 
+       the auxiliary variables composing C-program alphabet. Under this execution function
+       we consider only \emph{stable} initial state ie., normal initial state. 
+       Since Simpl semantics is defined only for initial normal state, using this semantics
+       will allow for an equivalent semantics as the one of Simpl language.*}
+
+abbreviation
+ "Simpl P \<equiv> C3(true \<turnstile> (P))"
+
+subsection{*Control flow statements*}
+
+text{*In the sequel we introduce the control-flow statements for C programming language.*}
+
+definition skip_c :: "('t::ordered_cancel_monoid_diff,'f,'\<alpha>) hrel_cp" ("SKIP")
+where [urel_defs]:"SKIP = Simpl ($tr\<acute> =\<^sub>u $tr \<and> \<not>$wait\<acute> \<and> \<not>$abrupt\<acute> \<and> $fault\<acute> =\<^sub>u \<guillemotleft>None\<guillemotright> \<and> \<lceil>II\<rceil>\<^sub>C)"
+
+definition stuck_c :: "('t::ordered_cancel_monoid_diff,'f,'\<alpha>) hrel_cp" ("STUCK")
+where [urel_defs]: "STUCK = (\<not>$ok\<acute> \<or> $wait\<acute> \<or> $abrupt\<acute> \<or> $fault\<acute> \<noteq>\<^sub>u \<guillemotleft>None\<guillemotright>)"
+
+definition assigns_c :: "'\<alpha> usubst \<Rightarrow> ('t::ordered_cancel_monoid_diff,'f,'\<alpha>) hrel_cp" ("\<langle>_\<rangle>\<^sub>C")
+where [urel_defs]: "assigns_c \<sigma> = 
+                    C3(\<lceil>true\<rceil>\<^sub>D \<turnstile> ($tr\<acute> =\<^sub>u $tr \<and> \<not>$wait\<acute> \<and> \<not>$abrupt\<acute> \<and> $fault\<acute> =\<^sub>u \<guillemotleft>None\<guillemotright> \<and> \<lceil>\<langle>\<sigma>\<rangle>\<^sub>a\<rceil>\<^sub>C))"
+
+subsection{*THROW*}
+
+definition throw_c :: "('t::ordered_cancel_monoid_diff,'f,'\<alpha>) hrel_cp" ("THROW")
+where [urel_defs]: "THROW = Simpl ($tr\<acute> =\<^sub>u $tr \<and> \<not>$wait\<acute> \<and> $abrupt\<acute> \<and> $fault\<acute> =\<^sub>u \<guillemotleft>None\<guillemotright> \<and> \<lceil>II\<rceil>\<^sub>C)"
+
+subsection{*Conditional*}
+
+abbreviation If_c::"'\<alpha> cond \<Rightarrow>('t::ordered_cancel_monoid_diff,'f,'\<alpha>) hrel_cp \<Rightarrow> ('t,'f,'\<alpha>) hrel_cp \<Rightarrow> 
+                    ('t,'f,'\<alpha>) hrel_cp" ("bif (_)/ then (_) else (_) eif")where
+  "If_c b P Q \<equiv> (P \<triangleleft> \<lceil>b\<rceil>\<^sub>C\<^sub>< \<triangleright> Q)"
+
+subsection{*GUARD*}
+
+abbreviation guard_c :: "'f \<Rightarrow> '\<alpha> cond \<Rightarrow> ('t::ordered_cancel_monoid_diff,'f,'\<alpha>) hrel_cp"  
+where "guard_c f b \<equiv> (bif b 
+                        then SKIP 
+                        else Simpl ($tr\<acute> =\<^sub>u $tr \<and> \<not>$wait\<acute> \<and> \<not>$abrupt\<acute> \<and> $fault\<acute> =\<^sub>u \<guillemotleft>Some f\<guillemotright> \<and> \<lceil>II\<rceil>\<^sub>C) 
+                      eif)"
+
+subsection{*Synchronisation*}
+
+abbreviation sync_c :: "'\<alpha> cond \<Rightarrow> ('t::ordered_cancel_monoid_diff,'f,'\<alpha>) hrel_cp"  
+where "sync_c b \<equiv> (bif b 
+                     then SKIP 
+                     else Simpl ($tr\<acute> =\<^sub>u $tr \<and> $wait\<acute> \<and> \<not>$abrupt\<acute> \<and> $fault\<acute> =\<^sub>u \<guillemotleft>None\<guillemotright> \<and> \<lceil>II\<rceil>\<^sub>C) 
+                   eif)"
+
+subsection{*assert and assume*}
+
+definition rassume_c :: "'\<alpha> upred \<Rightarrow> ('t::ordered_cancel_monoid_diff,'f,'\<alpha>) hrel_cp" ("_\<^sup>\<top>\<^sup>C" [999] 999) where
+[urel_defs]: "rassume_c c = (bif c then SKIP else \<top>\<^sub>D eif)"
+
+definition rassert_c :: "'\<alpha> upred \<Rightarrow> ('t::ordered_cancel_monoid_diff,'f,'\<alpha>) hrel_cp" ("_\<^sub>\<bottom>\<^sub>C" [999] 999) where
+[urel_defs]: "rassert_c c = (bif c then SKIP else \<bottom>\<^sub>D eif)"
+
+subsection{*Exceptions*}
+
+abbreviation catch_c :: "('t::ordered_cancel_monoid_diff,'f,'\<alpha>) hrel_cp \<Rightarrow> ('t,'f,'\<alpha>) hrel_cp \<Rightarrow> 
+                         ('t,'f,'\<alpha>) hrel_cp" ("try (_) catch /(_) end")
+where "try P catch Q end \<equiv> (P ;; ((abrupt:== (\<not> &abrupt) ;;Q) \<triangleleft> $abrupt \<triangleright> II))"
+
+subsection{*Scoping*}
+
+definition block_c ("bob INIT (_) BODY /(_) RESTORE /(_) RETURN/(_) eob") where
+[urel_defs]:
+  "bob INIT init BODY body RESTORE restore RETURN return eob= 
+    (Abs_uexpr (\<lambda>(s, s'). 
+     \<lbrakk>init ;; body ;; Abs_uexpr (\<lambda>(t, t').
+                       \<lbrakk>(abrupt:== (\<not> &abrupt) ;;restore (s, s') (t, t');; THROW) \<triangleleft> $abrupt \<triangleright> II;; 
+         restore (s, s') (t, t');; return(s, s') (t, t')\<rbrakk>\<^sub>e (t, t'))\<rbrakk>\<^sub>e (s, s')))" 
+
+subsection{*Loops*}
+purge_notation while ("while\<^sup>\<top> _ do _ od")
+
+definition While :: "'\<alpha> cond \<Rightarrow> ('t::ordered_cancel_monoid_diff,'f,'\<alpha>) hrel_cp \<Rightarrow> 
+                     ('t,'f,'\<alpha>) hrel_cp" ("while\<^sup>\<top> _ do _ od") where
+"While b C = (\<nu> X \<bullet> bif b then (C ;; X) else SKIP eif)"
+
+purge_notation while_top ("while _ do _ od")
+
+abbreviation While_top :: "'\<alpha> cond \<Rightarrow> ('t::ordered_cancel_monoid_diff,'f,'\<alpha>) hrel_cp \<Rightarrow>  
+                           ('t,'f,'\<alpha>) hrel_cp" ("while _ do _ od") where
+"while b do P od \<equiv> while\<^sup>\<top> b do P od"
+
+purge_notation while_bot ("while\<^sub>\<bottom> _ do _ od")
+
+definition While_bot :: "'\<alpha> cond \<Rightarrow> ('t::ordered_cancel_monoid_diff,'f,'\<alpha>) hrel_cp \<Rightarrow> 
+                         ('t,'f,'\<alpha>) hrel_cp" ("while\<^sub>\<bottom> _ do _ od") where
+"while\<^sub>\<bottom> b do P od =  (\<mu> X \<bullet> bif b then (P ;; X) else SKIP eif)"
+
+subsection{*While-loop inv*}
+text {* While loops with invariant decoration *}
+
+purge_notation while_inv ("while _ invr _ do _ od" 70)
+
+definition While_inv :: "'\<alpha> cond \<Rightarrow> '\<alpha> cond \<Rightarrow> ('t::ordered_cancel_monoid_diff,'f,'\<alpha>) hrel_cp \<Rightarrow> 
+                         ('t,'f,'\<alpha>) hrel_cp" ("while _ invr _ do _ od" 70) where
+"while b invr p do S od = while b do S od"
+
+declare While_def [urel_defs]
+declare While_inv_def [urel_defs]
+declare While_bot_def [urel_defs]
+
+
+syntax
+  "_assignmentc" :: "svid_list \<Rightarrow> uexprs \<Rightarrow> logic"  (infixr "\<Midarrow>" 55)
+
+translations
+  "_assignmentc xs vs" => "CONST assigns_c (_mk_usubst (CONST id) xs vs)"
+  "x \<Midarrow> v" <= "CONST assigns_c (CONST subst_upd (CONST id) (CONST svar x) v)"
+  "x \<Midarrow> v" <= "CONST assigns_c (CONST subst_upd (CONST id) x v)"
+  "x,y \<Midarrow> u,v" <= "CONST assigns_c (CONST subst_upd (CONST subst_upd (CONST id) (CONST svar x) u) (CONST svar y) v)"
+
+end
